feat: pure step

CollapsingTowers/TwoLevelBasic/SmallStep.lean
@@ -421,9 +421,53 @@ inductive stepn : Expr → Expr → Prop
   | refl : ∀ e, stepn e e
   | multi : ∀ e₀ e₁ e₂, stepn e₀ e₁ → step e₁ e₂ → stepn e₀ e₂
 
-theorem stepn_trans : ∀ e₀ e₁ e₂, stepn e₀ e₁ → stepn e₁ e₂ → stepn e₀ e₂ := by
+inductive pure_step : Expr → Expr → Prop where
+  | pure_step𝕄 : ∀ M e₀ e₁, ctx𝕄 0 M → lc e₀ → head𝕄 e₀ e₁ → pure_step M⟦e₀⟧ M⟦e₁⟧
+
+inductive pure_stepn : Expr → Expr → Prop
+  | refl : ∀ e, pure_stepn e e
+  | multi : ∀ e₀ e₁ e₂, pure_stepn e₀ e₁ → pure_step e₁ e₂ → pure_stepn e₀ e₂
+
+theorem pure_step_impl_step : ∀ e₀ e₁, pure_step e₀ e₁ → step e₀ e₁ :=
+  by
+  intros e₀ e₁ Hstep
+  cases Hstep
+  case pure_step𝕄 HM Hlc Hhead =>
+    apply step_lvl.step𝕄
+    apply HM; apply Hlc; apply Hhead
+
+theorem pure_stepn_impl_stepn : ∀ e₀ e₁, pure_stepn e₀ e₁ → stepn e₀ e₁ :=
+  by
+  intros e₀ e₁ Hstepn
+  induction Hstepn
+  case refl => apply stepn.refl
+  case multi H IH =>
+    apply stepn.multi
+    apply IH; apply pure_step_impl_step; apply H
+
+theorem pure_stepn_trans : ∀ e₀ e₁ e₂, pure_stepn e₀ e₁ → pure_stepn e₁ e₂ → pure_stepn e₀ e₂ :=
+  by
   intros e₀ e₁ e₂ Hstep₀ Hstep₁
   induction Hstep₁
   case refl => apply Hstep₀
   case multi H IH =>
-    apply stepn.multi; apply IH; apply H
+    apply pure_stepn.multi; apply IH; apply H
+
+theorem pure_step_at𝔹 : ∀ B e₀ e₁, ctx𝔹 B → pure_step e₀ e₁ → pure_step B⟦e₀⟧ B⟦e₁⟧ :=
+  by
+  intros B e₀ e₁ HB Hstep
+  cases Hstep
+  case pure_step𝕄 M _ _ HM Hlc Hhead =>
+    rw [ctx_comp B M]
+    apply pure_step.pure_step𝕄
+    apply ctx𝕄.cons𝔹; apply HB; apply HM
+    apply Hlc; apply Hhead
+
+theorem pure_stepn_at𝔹 : ∀ B e₀ e₁, ctx𝔹 B → pure_stepn e₀ e₁ → pure_stepn B⟦e₀⟧ B⟦e₁⟧ :=
+  by
+  intros B e₀ e₁ HB Hstepn
+  induction Hstepn
+  case refl => apply pure_stepn.refl
+  case multi H IH =>
+    apply pure_stepn.multi
+    apply IH; apply pure_step_at𝔹; apply HB; apply H
